\documentclass{homework}

\linespread{1.2}

\usepackage[T1]{fontenc}\usepackage{palatino}
\usepackage{amssymb,amsmath,amsthm,mathtools}
\usepackage[english]{babel}
\usepackage[utf8]{inputenc}
\usepackage[babel]{csquotes}
\usepackage[pdftex]{hyperref}
\usepackage{enumitem}
\usepackage[usenames,dvipsnames,table,xcdraw]{xcolor}

\usepackage{graphicx} 
\usepackage{verbatim} % Commenti in blocco con \begin{comment}
\usepackage{bm}
\usepackage[font={small,it}]{caption}
\usepackage{subcaption}
\usepackage{geometry}
\usepackage{array}
\usepackage{enumitem}
\setlist[enumerate]{label*=\arabic*.}
	
\usepackage{algorithm}
\usepackage[noend]{algpseudocode}
\usepackage{listings}

\definecolor{mygraybackground}{gray}{0.95}

% Define the R listings to write code
\lstset{
  language=R,
  basicstyle=\scriptsize\ttfamily, 
  numbers=left,
  numberstyle=\small\ttfamily\color{Gray},
  numbersep=10pt,
  backgroundcolor=\color{mygraybackground},
  showstringspaces=false,
  showtabs=false,
  tabsize=3,
  breaklines=true,
  captionpos=b,   
  keywordstyle=\color{black},
  commentstyle=\color{ForestGreen},
}

\makeatletter
\def\BState{\State\hskip-\ALG@thistlm}
\makeatother

% Simbolo iid
\newcommand\iid{\stackrel{\mathclap{\normalfont\tiny\mbox{iid}}}{\sim}}
% Simbolo ind
\newcommand\ind{\stackrel{\mathclap{\normalfont\tiny\mbox{ind}}}{\sim}}

\title{SDS 385: Homework 2}
\author{G.~Paulon}

\begin{document}

\makeatletter
\begin{titlepage}
	\vspace*{\fill}
	\centering
	{\huge \@title \par}
	\vskip0.5cm
	{\large \@author \par}
	\vskip0.5cm
	{\large \today \par}
	\vspace*{\fill}
\end{titlepage}
\makeatother

\newpage 
\mbox{}
\thispagestyle{empty}
\newpage

\setcounter{page}{1}

\problem{SGD for logistic regression}

\begin{enumerate}[label=(\Alph*)]

\item In part (A) of the last homework we proved that the gradient of the negative log-likelihood can be expressed as
\begin{equation*}
\nabla l(\beta) = - \sum_{i=1}^n \left\lbrace x_i (y_i - m_i w_i) \right\rbrace = \sum_{i=1}^n g_i (\beta)
\end{equation*}
where
\begin{equation*}
g_i (\beta) = x_i (y_i - m_i w_i) = x_i (y_i - \hat{y}_i)
\end{equation*}
and
\begin{equation*}
\hat{y}_i = \mathbb{E} (y_i | \beta) = m_i w_i (\beta) = m_i \frac{1}{1+\exp(-x_i^T \beta)}.
\end{equation*}

\item

\item

\item

\item

\end{enumerate}


\end{document}
